src/single_conf_message/DY.Example.SingleConfMessage.SecurityProperties.fst
@@ -58,20 +58,19 @@ let secret_secrecy_receiver tr sender receiver secret =
 // We can also not authenticate the sender because
 // the attacker could write an arbitrary sender in
 // the message. The only thing we can prove is
-// that if the secret is not publisable, the
-// sender contained in the message triggered an
-// event.
+// that if the secret is not publisable, there
+// exists a sender that triggered the send event.
 val sender_authentication:
   tr:trace ->
-  sender:principal -> receiver:principal ->
+  receiver:principal ->
   secret:bytes ->
   Lemma
   (requires
     trace_invariant tr /\
-    event_triggered tr receiver (ReceiverReceivedMsg sender receiver secret (compute_message secret))
+    event_triggered tr receiver (ReceiverReceivedMsg receiver secret (compute_message secret))
   )
   (ensures
-    event_triggered tr sender (SenderSendMsg sender receiver secret) \/
+    (exists sender. event_triggered tr sender (SenderSendMsg sender receiver secret)) \/
     is_publishable tr (compute_message secret)
     // We cannot prove `is_corrupt tr
     // (principal_label sender)` because the
@@ -80,7 +79,7 @@ val sender_authentication:
     // choose an arbitrary sender for the sender
     // field.
   )
-let sender_authentication tr sender receiver secret = ()
+let sender_authentication tr receiver secret = ()
 
 (*
 
