src/single_conf_and_auth_message/DY.Example.SingleConfAuthMessage.SecurityProperties.fst
@@ -1,0 +1,60 @@
+module DY.Example.SingleConfAuthMessage.SecurityProperties
+
+open Comparse
+open DY.Core
+open DY.Lib
+open DY.Example.SingleConfAuthMessage.Protocol.Total.Proof
+open DY.Example.SingleConfAuthMessage.Protocol.Stateful
+open DY.Example.SingleConfAuthMessage.Protocol.Stateful.Proof
+
+#set-options "--fuel 0 --ifuel 0 --z3rlimit 10  --z3cliopt 'smt.qi.eager_threshold=100'"
+
+// Since the message is authenticated we can prove on the receiver side that
+// either the sender triggered a send event or the sender is corrupt.
+val sender_authentication:
+  tr:trace -> i:timestamp ->
+  sender:principal -> receiver:principal ->
+  secret:bytes ->
+  Lemma
+  (requires
+    trace_invariant tr /\
+    event_triggered_at tr i receiver (ReceiverReceivedMsg sender receiver secret)
+  )
+  (ensures
+    event_triggered tr sender (SenderSendMsg sender receiver secret) \/
+    is_corrupt tr (principal_label sender)
+  )
+let sender_authentication tr i sender receiver secret = ()
+
+
+// Secrecy property of the secret from the sender's perspective
+val secret_secrecy_sender:
+  tr:trace -> sender:principal -> receiver:principal -> secret:bytes ->
+  Lemma
+  (requires
+    trace_invariant tr /\
+    attacker_knows tr secret /\
+    (exists sess_id. state_was_set tr sender sess_id (SenderState receiver secret))
+  )
+  (ensures
+    is_corrupt tr (principal_label sender) \/ is_corrupt tr (principal_label receiver)
+  )
+let secret_secrecy_sender tr sender receiver secret =
+  attacker_only_knows_publishable_values tr secret;
+  ()
+
+// Since the message is authenticated we can prove from the receiver's perspective that if the attacker knows the secret, either the sender or the receiver is corrupt.
+val secret_secrecy_receiver:
+  tr:trace -> sender:principal -> receiver:principal -> secret:bytes ->
+  Lemma
+  (requires
+    trace_invariant tr /\
+    attacker_knows tr secret /\
+    event_triggered tr receiver (ReceiverReceivedMsg sender receiver secret)
+  )
+  (ensures
+    is_corrupt tr (principal_label sender) \/ is_corrupt tr (principal_label receiver)
+  )
+let secret_secrecy_receiver tr sender receiver secret =
+  attacker_only_knows_publishable_values tr secret;
+  ()
